execution/tests/CongressGens.v
@@ -1,0 +1,138 @@
+From ConCert Require Import Blockchain LocalBlockchain Congress.
+From ConCert Require Import Serializable.
+From ConCert Require Import BoundedN ChainedList.
+From ConCert.Execution.QCTests Require Import ChainGens TestUtils ChainPrinters CongressPrinters.
+
+Require Import ZArith Strings.Ascii Strings.String.
+
+From QuickChick Require Import QuickChick. Import QcNotation.
+From ExtLib.Structures Require Import Functor Applicative.
+Require Export ExtLib.Structures.Monads.
+Export MonadNotation. Open Scope monad_scope.
+From Coq Require Import List. Import ListNotations.
+From Coq Require Import Strings.BinaryString.
+From Coq Require Import Morphisms.
+From Coq Require Import Program.Basics.
+Require Import Containers.
+
+Notation "f 'o' g" := (compose f g) (at level 50).
+
+(* ChainGens for the types defined in the Congress contract *)
+
+Definition LocalChainBase : ChainBase := ChainGens.LocalChainBase.
+
+
+Definition gRulesSized (n : nat) : G Rules :=
+  vote_count <- gZPositiveSized n ;;
+  margin <- liftM Z.of_nat (gIntervalNat n (2 * n)) ;;
+  liftM (build_rules vote_count margin) arbitrary.  
+
+Instance genRulesSized : GenSized Rules :=
+{|
+  arbitrarySized := gRulesSized
+|}.
+
+Instance genSetupSized : GenSized Setup := 
+{|
+  arbitrarySized n := liftM build_setup (arbitrarySized n)
+|}.
+
+Definition gCongressAction' {ctx : ChainContext LocalChainBase}
+                           (gMsg : G SerializedValue) 
+                           : G CongressAction :=
+  (* We only want to generate positive amounts for now, but could be worth looking into *)
+  freq [
+    (1, liftM2 cact_transfer (ctx_gAccountAddr ctx) gZPositive);
+    (1, liftM3 cact_call (ctx_gContractAddr ctx) gZPositive gMsg)
+  ].
+
+Sample (ctx <- @arbitrarySized _ genLocalBaseGens 1 ;; @gCongressAction' ctx arbitrary).
+
+
+
+Definition gMsgSimple (ctx : ChainContext LocalChainBase) : G Msg := 
+  freq [
+    (1, liftM transfer_ownership (ctx_gAccountAddr ctx)) ;
+    (1, liftM change_rules arbitrary) ;
+    (2, liftM add_member (ctx_gAccountAddr ctx)) ;
+    (2, liftM remove_member (ctx_gAccountAddr ctx)) ;
+    (2, liftM vote_for_proposal arbitrary) ;
+    (2, liftM vote_against_proposal arbitrary) ;
+    (2, liftM retract_vote arbitrary) ;
+    (2, liftM finish_proposal arbitrary)
+  ].
+Definition gMsg' : G Msg := 
+  ctx <- arbitrary ;; gMsgSimple ctx.
+
+Sample gMsg'.
+
+
+Sample (ctx <- @arbitrarySized _ genLocalBaseGens 1 ;; 
+        ctx_gAccountAddr ctx).
+
+
+Fixpoint gMsgSized (ctx : ChainContext LocalChainBase) (n : nat) : G Msg :=
+  let default := liftM transfer_ownership (ctx_gAccountAddr ctx) in
+  match n with
+    | 0 => gMsgSimple ctx
+    | S n' => freq [
+        (1, (* TODO: fix weight. should be roughly 1:8*)
+        (* recurse. Msg is converted to a SerializedType using 'serialize' *)
+        (* This makes it possible to create proposals about proposals about proposals etc... *)
+        congressActions <- listOf (@gCongressAction' ctx (liftM serialize (gMsgSized ctx n'))) ;;
+        returnGen (create_proposal congressActions)) ;
+        (7, gMsgSimple ctx)
+      ]
+  end.
+
+Sample (ctx <- arbitrary ;; @gMsgSized ctx 1).
+
+Example ex_simple_msg : Msg := create_proposal [cact_call zero_address 1%Z (serialize 123)].
+Example ex_msg : Msg := create_proposal [cact_call zero_address 0%Z (serialize ex_simple_msg)].
+Compute ((show o deserialize o serialize) ex_simple_msg).
+Compute (show ex_msg). 
+
+
+
+Definition gCongressActionSized {ctx : ChainContext LocalChainBase}
+                                (n : nat)
+                                : G CongressAction 
+                                := @gCongressAction' ctx (liftM serialize (@gMsgSized ctx n)).
+
+
+Sample (ctx <- arbitrary ;; gMsgSized ctx 2).
+
+Example ex_call_congress_action := ctx <- arbitrary ;; 
+                                   liftM (cact_call zero_address 0%Z) (liftM serialize (gMsgSized ctx 2) ).
+Sample ex_call_congress_action.
+
+Definition gProposalSized {ctx : ChainContext LocalChainBase} 
+                          (n : nat)
+                          : G Proposal :=
+  bound <- arbitrarySized n ;;
+  actions <- vectorOf bound (@gCongressActionSized ctx n) ;;
+  let nr_votes := length (ctx_accounts ctx) in
+  vote_vals <- vectorOf nr_votes arbitrary ;;
+  votes <- gFMapFromInput (ctx_accounts ctx) vote_vals ;;
+  vote_result <- gZPositive ;;
+  proposed_in <- arbitrary ;;
+  returnGen (build_proposal actions votes vote_result proposed_in).
+
+Sample (ctx <- arbitrary ;; @gProposalSized ctx 1).
+
+
+Definition gStateSized {ctx : ChainContext LocalChainBase} 
+                       (n : nat) 
+                       : G Congress.State :=
+  let nr_accounts := length (ctx_accounts ctx) in
+  default_addr <- (ctx_gAccountAddr ctx) ;;
+  owner <- elems_ default_addr (ctx_accounts ctx) ;;
+  rules <- arbitrarySized nr_accounts ;;
+  proposalIds <- vectorOfCount 0 n ;;
+  proposals <- vectorOf n (@gProposalSized ctx n) ;;
+  proposals_map <- gFMapFromInput proposalIds proposals ;;
+  next_proposal_id <- arbitrary ;; (* TODO: ensure valid proposal Id*)
+  unit_list <- (vectorOf nr_accounts (returnGen tt)) ;;
+  members <- gFMapFromInput (ctx_accounts ctx) unit_list ;;
+  returnGen (build_state owner rules proposals_map next_proposal_id members).
+
