execution/tests/CongressPrinters.v
@@ -1,0 +1,90 @@
+From ConCert Require Import Blockchain LocalBlockchain Congress.
+From ConCert Require Import Serializable.
+From ConCert Require Import BoundedN ChainedList.
+From ConCert.Execution.QCTests Require Import ChainGens TestUtils ChainPrinters.
+
+Require Import ZArith Strings.Ascii Strings.String.
+
+From QuickChick Require Import QuickChick. Import QcNotation.
+From ExtLib.Structures Require Import Functor Applicative.
+Require Export ExtLib.Structures.Monads.
+Export MonadNotation. Open Scope monad_scope.
+From Coq Require Import List. Import ListNotations.
+From Coq Require Import Strings.BinaryString.
+From Coq Require Import Morphisms.
+From Coq Require Import Program.Basics.
+Require Import Containers.
+Notation "f 'o' g" := (compose f g) (at level 50).
+Definition LocalChainBase : ChainBase := ChainGens.LocalChainBase.
+Open Scope string_scope.
+
+
+Instance showRules : Show Rules :=
+{|
+  show r := 
+    "Rules{"
+    ++ "min_vote_count_permille: " ++ show (min_vote_count_permille r) ++ sep
+    ++ "margin_needed_permille: " ++ show (margin_needed_permille r) ++ sep
+    ++ "debating_period_in_blocks: " ++ show (debating_period_in_blocks r) 
+    ++ "}"
+|}.
+
+
+(* TODO: fix printing for msg of type SerializedValue such that it works whenever it is serialized from type Msg *)
+Instance showCongressAction : Show CongressAction :=
+{|
+  show ca :=
+    match ca with
+    | cact_transfer to amount => "(transfer: " ++ show to ++ sep ++ show amount ++ ")"
+    | cact_call to amount msg => "(call: " ++ show to ++ sep ++ show amount ++ sep ++  show msg ++ ")" 
+    end
+|}.
+
+Instance showProposal : Show Proposal :=
+{|
+  show p :=
+    "Proposal{"
+    ++ "actions: " ++ show (actions p) ++ sep
+    ++ "votes: " ++ show (votes p) ++ sep
+    ++ "vote_result: " ++ show (vote_result p) ++ sep
+    ++ "proposed_in: " ++ show (proposed_in p) ++ sep
+    ++ "}" ++ newline
+|}.
+
+Instance showSetup : Show Setup :=
+{|
+  show := show o setup_rules
+|}.
+
+
+Definition string_of_Msg (m : Msg) : string :=
+  match m with
+    | transfer_ownership addr => "(transfer_ownership " ++  show addr ++ ")"
+    | change_rules rules => "(change_rules " ++ show rules ++ ")"
+    | add_member addr => "(add_member " ++ show addr ++ ")"
+    | remove_member addr => "(remove_member " ++ show addr ++ ")"
+    | create_proposal actions => "(create_proposal " ++ show actions ++ ")"
+    (* | create_proposal actions => "(create_proposal " ++  String.concat "; " (map (@show _ (@showCongressAction showSer) ) actions) ++ ")" *)
+    | vote_for_proposal proposalId => "(vote_for_proposal " ++ show proposalId ++ ")"
+    | vote_against_proposal proposalId => "(vote_against_proposal " ++ show proposalId ++ ")"
+    | retract_vote proposalId => "(retract_vote " ++ show proposalId ++ ")"
+    | finish_proposal proposalId => "(finish_proposal " ++ show proposalId ++ ")"
+  end.
+
+Instance showMsg : Show Msg :=
+{|
+  show := string_of_Msg
+|}.
+
+
+Instance showState : Show Congress.State :=
+{|
+  show s := "State{" 
+            ++ "owner: " ++ show (owner s) ++ sep
+            ++ "rules: " ++ show (state_rules s) ++ sep
+            ++ "proposals: " ++ show (proposals s) ++ sep
+            ++ "next_proposal_id: " ++ show (next_proposal_id s) ++ sep
+            ++ "members: " ++ show (members s) ++ "}"
+|}.
+
+Close Scope string_scope.
